Quotes with Pi finished

theories/Quotes.v
@@ -1,13 +1,19 @@
 
-Set Primitive Projections.
 Set Universe Polymorphism.
-Set Printing Universes.
+(* Set Printing Universes. *)
 
 Section Notations.
 
-(* Inductive eq@{i} (A : Type@{i}) (a : A) : A -> Type@{i} :=  eq_refl : eq A a a. *)
-(* Arguments eq {A} _ _. *)
-(* Arguments eq_refl {A} a. *)
+(** * Pi *)
+
+Axiom Π@{i j} : forall (A : Type@{i}) (B : A -> Type@{j}), Type@{max(i,j)}.
+Axiom λ@{i j} : forall {A : Type@{i}} {B : A -> Type@{j}} (t : forall x, B x), Π A B. 
+Axiom App@{i j} : forall {A : Type@{i}} (B : A -> Type@{j}) (t : Π A B) (u : A), B u.
+
+Notation "A ⇒ B" := (Π A (fun _ : A => B)) (at level 20, right associativity).
+Notation "t $ u" := (App _ t u) (at level 19, left associativity).
+
+(** * Eq *)
 
 Axiom eq@{i} : forall {A : Type@{i}} (a : A), A -> Type@{i}.
 Axiom eq_refl@{i} : forall {A : Type@{i}} (a : A), eq a a.
@@ -21,54 +27,18 @@ Axiom J@{i j} : forall {A : Type@{i}} {u} (P : forall (x : A), u = x -> Type@{j}
 Axiom Jβ@{i j} : forall {A : Type@{i}} {u} (P : forall (x : A), u = x -> Type@{j})
            (w : P u (@eq_refl A u)), J P (@eq_refl A u) w = w.
 Axiom K@{i} : forall {A : Type@{i}} {x : A} (p : x = x), p = 1.
-Axiom funext@{i j ij} : forall {A : Type@{i}} {B : A -> Type@{j}} {f g : forall (x : A), B x},
-    (forall x, f x = g x) -> eq@{ij} f g.
+
+Axiom β@{i j} : forall {A : Type@{i}} {B : A -> Type@{j}} (t : forall x, B x) (u : A),
+    (λ t) $ u = t u.
+Axiom funext@{i j ij} : forall {A : Type@{i}} {B : A -> Type@{j}} {f g : Π A B},
+    (forall x, f $ x = g $ x) -> eq@{ij} f g.
 
 Definition transport@{i j} {A : Type@{i}} (P : A -> Type@{j}) {x y : A} (p : x = y) (u : P x) : P y
   := J (fun y _ => P y) p u.
 
 Notation "p # x" := (transport _ p x) (right associativity, at level 65, only parsing).
 
-Definition inverse@{i} {A : Type@{i}} {x y : A} (p : x = y) : y = x
-  := transport (fun x' => x' = x) p 1.
-
-Definition concat@{i} {A : Type@{i}} {x y z : A} (p : x = y) (q : y = z) : x = z
-  := transport (eq x) q p.
-
-Notation "p @ q" := (concat p q) (at level 20).
-Notation "p ^" := (inverse p) (at level 3, format "p '^'").
-
-Definition ap@{i j} {A : Type@{i}} {B : Type@{j}} (f : A -> B) {x y} (p : x = y)
-  : f x = f y
-  := transport (fun y => f x = f y) p 1.
-
-Definition coe@{i i1} {A B : Type@{i}} (p : eq@{i1} A B) : A -> B
-  := fun x => transport (fun T => T) p x.
-(* Axiom coe@{i i1} : forall {A B : Type@{i}} (p : eq@{i1} A B), A -> B. *)
-
-Definition transportβ@{i j} {A : Type@{i}} (P : A -> Type@{j}) {x} (u : P x)
-  : transport@{i j} P 1 u = u
-  := Jβ@{i j} (fun x _ => P x)u.
-
-Definition coeβ@{i i1} {A : Type@{i}} (x : A)
-  : coe@{i i1} 1 x = x
-  := transportβ (fun T => T) x.
-(* . Admitted. *)
-
-Tactic Notation "etransitivity" := refine (_ @ _).
-Tactic Notation "symmetry" := refine (_^).
-Tactic Notation "reflexivity" := exact 1.
-
-
-
-
-(* Record sigT@{i j} {A : Type@{i}} (P : A -> Type@{j}) : Type@{max(i,j)} := existT *)
-(*   { projT1 : A ; projT2 : P projT1 }. *)
-
-(* Arguments existT {A} P _ _. *)
-(* Arguments projT1 {A P} _. *)
-(* Arguments projT2 {A P} _. *)
-
+(** * Sigma *)
 
 Axiom sigT@{i j} : forall {A : Type@{i}} (P : A -> Type@{j}), Type@{max(i,j)}.
 Axiom existT@{i j} : forall {A : Type@{i}} (P : A -> Type@{j}) (x : A) (y : P x), sigT P.
@@ -91,6 +61,38 @@ Axiom projT2β@{i j} : forall {A : Type@{i}} (P : A -> Type@{j}) x y,
 Axiom Ση@{i j ij} : forall {A : Type@{i}} (P : A -> Type@{j}) (z : {x : A & P x}),
     eq@{ij} (z.1; z.2) z.
 
+(** * Defined constants *)
+
+Definition inverse@{i} {A : Type@{i}} {x y : A} (p : x = y) : y = x
+  := transport (fun x' => x' = x) p 1.
+
+Definition concat@{i} {A : Type@{i}} {x y z : A} (p : x = y) (q : y = z) : x = z
+  := transport (eq x) q p.
+
+Notation "p @ q" := (concat p q) (at level 20).
+Notation "p ^" := (inverse p) (at level 3, format "p '^'").
+
+Definition ap@{i j} {A : Type@{i}} {B : Type@{j}} (f : A -> B) {x y} (p : x = y)
+  : f x = f y
+  := transport (fun y => f x = f y) p 1.
+
+Definition coe@{i i1} {A B : Type@{i}} (p : eq@{i1} A B) : A -> B
+  := fun x => transport (fun T => T) p x.
+
+Definition transportβ@{i j} {A : Type@{i}} (P : A -> Type@{j}) {x} (u : P x)
+  : transport@{i j} P 1 u = u
+  := Jβ@{i j} (fun x _ => P x)u.
+
+Definition coeβ@{i i1} {A : Type@{i}} (x : A)
+  : coe@{i i1} 1 x = x
+  := transportβ (fun T => T) x.
+
+Tactic Notation "etransitivity" := refine (_ @ _).
+Tactic Notation "transitivity" uconstr(y) := refine (@concat _ _ y _ _ _).
+Tactic Notation "symmetry" := refine (_^).
+Tactic Notation "reflexivity" := exact 1.
+
+
 Definition sigT_rect@{i j ij k} {A : Type@{i}} (P : A -> Type@{j})
            (Q : {x : A & P x} -> Type@{k})
            (H : forall x p, Q (existT P x p))
@@ -105,10 +107,9 @@ Definition sigT_rec@{i j k} {A : Type@{i}} (P : A -> Type@{j})
            (H : forall x, P x -> Q)
   : {x : A & P x} -> Q
   := fun z => H z.1 z.2.
-  (* := sigT_rect@{i j ij k} P (fun _ => Q) H. *)
 
 Tactic Notation "exists" uconstr(x) := refine (existT _ x _).
-
+Tactic Notation "eexists" := refine (existT _ _ _).
 
 
 Definition heq@{i i1} {A : Type@{i}} (a : A) {B : Type@{i}} (b : B) :=
@@ -154,10 +155,6 @@ Proof.
   etransitivity. symmetry; eassumption. apply coeβ.
 Defined.
 
-(* Opaque transport coe heq inverse concat coeβ coeβ'. *)
-(* Eval compute in heq_sym. *)
-
-
 Lemma heq_trans@{i i1} {A B C : Type@{i}} (a : A) (b : B) (c : C)
   : heq@{i i1} a b -> b ≅ c -> a ≅ c.
 Proof.
@@ -174,12 +171,90 @@ Proof.
   symmetry; apply coeβ.
 Defined.
 
+Notation "p E@ q" := (heq_trans _ _ _ p q) (at level 20).
+Notation "p ^E" := (heq_sym _ _ p) (at level 3, format "p '^E'").
+Notation "'E1'" := (heq_refl _).
+
+Tactic Notation "etransitivity" := refine (_ @ _) || refine (_ E@ _).
+Tactic Notation "transitivity" uconstr(y) := refine (@concat _ _ y _ _ _) || refine (@heq_trans _ _ _ _ y _ _ _).
+Tactic Notation "symmetry" := refine (_^) || refine (_^E).
+Tactic Notation "reflexivity" := exact 1 || exact E1.
+
+Tactic Notation "wrevert" ident(H) :=
+  revert H;
+  match goal with
+  | |- (forall x, ?G) => let X := fresh "X" in
+                  refine (fun X => App (fun x => G) _ X); clear X
+  end.
+Tactic Notation "wintro" ident(H) := apply λ; intro H.
+Tactic Notation "wdestruct" ident(e) :=
+  match type of e with
+  | _ = ?y => 
+  revert y e;
+    match goal with
+    | |- (forall y e, ?G) => let X := fresh in let Y := fresh in
+                      refine (fun X Y => J (fun y e => G) Y _); clear X Y
+    end end.
+
+Tactic Notation "wrevert" ident(H1) ident(H2) := wrevert H1; wrevert H2.
+Tactic Notation "wrevert" ident(H1) ident(H2) ident(H3) := wrevert H1; wrevert H2; wrevert H3.
+Tactic Notation "wrevert" ident(H1) ident(H2) ident(H3) ident(H4) := wrevert H1; wrevert H2; wrevert H3; wrevert H4.
+Tactic Notation "wrevert" ident(H1) ident(H2) ident(H3) ident(H4) ident(H5) := wrevert H1; wrevert H2; wrevert H3; wrevert H4; wrevert H5.
+Tactic Notation "wrevert" ident(H1) ident(H2) ident(H3) ident(H4) ident(H5) ident(H6) := wrevert H1; wrevert H2; wrevert H3; wrevert H4; wrevert H5; wrevert H6.
+Tactic Notation "wintro" ident(H1) ident(H2) := wintro H1; wintro H2.
+Tactic Notation "wintro" ident(H1) ident(H2) ident(H3) := wintro H1; wintro H2; wintro H3.
+Tactic Notation "wintro" ident(H1) ident(H2) ident(H3) ident(H4) := wintro H1; wintro H2; wintro H3; wintro H4.
+Tactic Notation "wintro" ident(H1) ident(H2) ident(H3) ident(H4) ident(H5) := wintro H1; wintro H2; wintro H3; wintro H4; wintro H5.
+Tactic Notation "wintro" ident(H1) ident(H2) ident(H3) ident(H4) ident(H5) ident(H6) := wintro H1; wintro H2; wintro H3; wintro H4; wintro H5; wintro H6.
+
+Notation "'app' B1" := (fun x => B1 $ x) (at level 12).
+
+Tactic Notation "beta" := refine (β _ _) || refine (β _ _)^.
+
+Tactic Notation "wrevert" ident(H) :=
+  revert H;
+  match goal with
+  | |- (forall x, ?G) => let X := fresh "X" in
+                  refine (fun X => App (fun x => G) _ X); clear X
+  end.
+Tactic Notation "wintro" ident(H) := apply λ; intro H.
+Tactic Notation "wdestruct" ident(e) :=
+  match type of e with
+  | _ = ?y => 
+  revert y e;
+    match goal with
+    | |- (forall y e, ?G) => let X := fresh in let Y := fresh in
+                      refine (fun X Y => J (fun y e => G) Y _); clear X Y
+    end end.
+
+Tactic Notation "wrevert" ident(H1) ident(H2) := wrevert H1; wrevert H2.
+Tactic Notation "wrevert" ident(H1) ident(H2) ident(H3) := wrevert H1; wrevert H2; wrevert H3.
+Tactic Notation "wrevert" ident(H1) ident(H2) ident(H3) ident(H4) := wrevert H1; wrevert H2; wrevert H3; wrevert H4.
+Tactic Notation "wrevert" ident(H1) ident(H2) ident(H3) ident(H4) ident(H5) := wrevert H1; wrevert H2; wrevert H3; wrevert H4; wrevert H5.
+Tactic Notation "wrevert" ident(H1) ident(H2) ident(H3) ident(H4) ident(H5) ident(H6) := wrevert H1; wrevert H2; wrevert H3; wrevert H4; wrevert H5; wrevert H6.
+Tactic Notation "wintro" ident(H1) ident(H2) := wintro H1; wintro H2.
+Tactic Notation "wintro" ident(H1) ident(H2) ident(H3) := wintro H1; wintro H2; wintro H3.
+Tactic Notation "wintro" ident(H1) ident(H2) ident(H3) ident(H4) := wintro H1; wintro H2; wintro H3; wintro H4.
+Tactic Notation "wintro" ident(H1) ident(H2) ident(H3) ident(H4) ident(H5) := wintro H1; wintro H2; wintro H3; wintro H4; wintro H5.
+Tactic Notation "wintro" ident(H1) ident(H2) ident(H3) ident(H4) ident(H5) ident(H6) := wintro H1; wintro H2; wintro H3; wintro H4; wintro H5; wintro H6.
+
+Notation "'app' B1" := (fun x => B1 $ x) (at level 12).
+
+Tactic Notation "beta" := refine (β _ _) || refine (β _ _)^.
+
 
 Definition heq_type_eq@{i i1} {A : Type@{i}} {u : A} {B : Type@{i}} {v : B}
   : heq@{i i1} u v -> A = B
   := projT1.
 
-Lemma heq_transport@{i i1} {T T' : Type@{i}} (p : T = T') (t : T)
+Lemma heq_transport {A} {B : A -> Type} {x x'} (p : x = x') (t : B x)
+  : t ≅ (p # t).
+Proof.
+  exists (ap B p). wdestruct p. etransitivity.
+  apply coeβ'. symmetry; apply transportβ.
+Defined.
+
+Lemma heq_coe@{i i1} {T T' : Type@{i}} (p : T = T') (t : T)
   : t ≅ coe@{i i1} p t.
 Proof.
   exists p. reflexivity.
@@ -197,21 +272,16 @@ Defined.
 
 Definition Pack@{i i1} (A1 A2 : Type@{i}) : Type@{i1}
   := exists (x1 : A1)(x2 : A2), heq@{i i1} x1 x2.
-(* . Admitted. *)
 Definition pack@{i i1} {A1 A2 : Type@{i}} (x1 : A1) (x2 : A2) (e: heq @{i i1} x1 x2)
   : Pack@{i i1} A1 A2
   := (x1; (x2; e)).
-(* . Admitted. *)
 Definition ProjT1@{i i1} {A1 A2 : Type@{i}} (z : Pack@{i i1} A1 A2) : A1
   := z.1.
-(* . Admitted. *)
 Definition ProjT2@{i i1} {A1 A2 : Type@{i}} (z : Pack@{i i1} A1 A2) : A2
   := z.2.1.
-(* . Admitted. *)
 Definition ProjTe@{i i1} {A1 A2 : Type@{i}} (z : Pack@{i i1} A1 A2)
   : heq@{i i1} (ProjT1 z) (ProjT2 z)
   := z.2.2.
-(* . Admitted. *)
 
 
 Definition transport_sigma_const@{i j ij} {X A : Type@{i}} {B : A -> X -> Type@{j}}
@@ -232,7 +302,6 @@ Defined.
 Definition ProjT1β@{i i1} {A1 A2 : Type@{i}} (x1 : A1) (x2 : A2) (e: x1 ≅ x2)
  : ProjT1 (pack@{i i1} x1 x2 e) = x1
   := projT1β _ _ _.
-(* . Admitted. *)
 
 Definition ProjT2β@{i i1} {A1 A2 : Type@{i}} (x1 : A1) (x2 : A2) (e: x1 ≅ x2)
  : ProjT2 (pack@{i i1} x1 x2 e) = x2.
@@ -243,95 +312,362 @@ Proof.
   refine (_ @ ap projT1 X @ projT1β _ _ _).
   symmetry; eapply projT1β.
 Defined.
-(* Admitted. *)
 
 (* Definition ProjTeβ@{i i1} {A1 A2 : Type@{i}} (x1 : A1) (x2 : A2) (e: x1 ≅ x2) *)
 (*  : ProjTe (pack@{i i1} x1 x2 e) ≅ e. *)
 
 
-Lemma heq_to_eq_fam@{i i1 j j1 j2 ij1} (A : Type@{i})
-      (B1 : A -> Type@{j}) (B2 : A -> Type@{j})
-      (hB : forall (p : Pack@{i i1} A A), heq@{j1 j2} (B1 (ProjT1 p)) (B2 (ProjT2 p)))
-  : eq@{ij1} B1 B2.
+
+Definition transport_Vp@{i j} {A : Type@{i}} (P : A -> Type@{j})
+           {x y} (p : x = y) (u : P x)
+  : p^ # (p # u) = u.
 Proof.
-  apply funext. intro x.
-  refine (_ @ heq_to_eq (hB (pack x x (heq_refl x))) @ _).
-  all: apply ap. symmetry; apply ProjT1β. apply ProjT2β.
+  wdestruct p. etransitivity. eapply ap. apply transportβ.
+  etransitivity. 2: eapply (transportβ P).
+  refine (ap (fun p => transport P p u) _). apply K.
 Defined.
 
-Lemma heq_to_eq_fam'@{i i1 i2 j j1 j2 ij1 k i1j2k} {A1 A2 : Type@{i}}
-      {B1 : A1 -> Type@{j}} {B2 : A2 -> Type@{j}}
-      (hA : heq@{i1 i2} A1 A2)
-      (hB : forall (p : Pack@{i i1} A1 A2), heq@{j1 j2} (B1 (ProjT1 p)) (B2 (ProjT2 p)))
-      (P : forall (A : Type@{i})(B : A -> Type@{j}), Type@{k})
-      (P1 : P A1 B1)
-  : P A2 B2.
+Definition projT2β'@{i j} {A : Type@{i}} (P : A -> Type@{j}) x (y : P x)
+  : (x; y).2 = (projT1β _ _ _)^ # y.
 Proof.
-  revert B2 hB. refine (transport@{i1 i1j2k} (fun A2: Type@{i} => forall B2 : A2 -> Type@{j}, (forall p : Pack@{i i1} A1 A2, B1 (ProjT1@{i i1} p) ≅ B2 (ProjT2@{i i1} p)) -> P A2 B2) (heq_to_eq hA) _).
-  intros B2 hB. refine (transport@{ij1 k} _ _ P1). apply funext; intro x.
-  refine (_ @ heq_to_eq (hB (pack x x (heq_refl x))) @ _).
-  all: apply ap. symmetry; apply ProjT1β. apply ProjT2β.
+  refine (_ @ ap (transport P _) (projT2β P x y)).
+  symmetry; apply transport_Vp.
 Defined.
+
+
+Axiom congΠ@{i j j1 ij ij1} : forall {A : Type@{i}}{B B': A -> Type@{j}},
+    (forall x, eq@{j1} (B x) (B' x)) -> @eq@{ij1} Type@{ij} (Π@{i j} A B) (Π@{i j} A B').
+
+Lemma congΠβ@{i i1 i2 j j1 j2 ij ij1 ij2} (A1 : Type@{i})
+      (B1 B2 : A1 -> Type@{j}) (f1 : Π A1 B1)
+      (hB : forall x, B1 x = B2 x)
+  : coe@{ij ij1} (congΠ@{i j j1 ij ij1} hB) f1
+    = λ@{i j} (fun x => coe (hB x) (f1 $ x)).
+Proof.
+Admitted.
 
 
 Lemma cong_prod@{i i1 i2 j j1 j2 ij ij1 ij2} (A1 A2 : Type@{i})
       (B1 : A1 -> Type@{j}) (B2 : A2 -> Type@{j})
       (hA : heq@{i1 i2} A1 A2)
       (hB : forall (p : Pack@{i i1} A1 A2), heq@{j1 j2} (B1 (ProjT1 p)) (B2 (ProjT2 p)))
-  : @heq@{ij1 ij2} Type@{ij} (forall x : A1, B1 x) Type@{ij} (forall y : A2, B2 y).
+  : @heq@{ij1 ij2} Type@{ij} (Π A1 B1) Type@{ij} (Π A2 B2).
 Proof.
-  refine (heq_to_eq_fam'@{i i1 i2 j j1 j2 ij1 ij2 ij2} hA hB (fun A2 B2 => @heq@{ij1 ij2} Type@{ij} (forall x : A1, B1 x) Type@{ij} (forall y : A2, B2 y)) _). eapply heq_refl.
+  apply heq_to_eq in hA. apply eq_to_heq.
+  pose (B2' := λ@{i j1} B2).
+  refine (@concat Type@{ij} _ (Π@{i j} A2 (app B2')) _ _ _).
+  2: apply congΠ@{i j j1 ij ij1}; intro x; apply (β@{i j1} B2 x).
+  assert (XX: Π@{ij1 ij1} _ (fun B2' => (Π@{ij1 ij1} (Pack@{i i1} A1 A2) (fun p => B1 (ProjT1@{i i1} p) ≅ B2' $ (ProjT2@{i i1} p))) ⇒ (@eq Type@{ij} (Π@{i j} A1 B1) (Π@{i j} A2 (fun x => B2' $ x))))). {
+    refine (transport (fun A2 => Π@{ij1 ij1} (A2 ⇒ Type@{j}) (fun B2' : A2 ⇒ Type@{j} => Π@{ij1 ij1} (Pack@{i i1} A1 A2) (fun p : Pack@{i i1} A1 A2 => B1 (ProjT1@{i i1} p) ≅ B2' $ ProjT2@{i i1} p) ⇒ (@eq Type@{ij} (Π@{i j} A1 B1) (Π@{i j} A2 (fun x : A2 => B2' $ x)))) ) hA _).
+    clear. apply λ; intro B2'.
+    apply λ; intro p.
+    eapply congΠ@{i j j1 ij ij1}.
+    intro x. pose proof (p $ (pack@{i i1} x x (heq_refl x))).
+    cbn in *. apply heq_to_eq in X. etransitivity. etransitivity.
+    2: exact X. all: apply ap.
+    symmetry. apply ProjT1β. apply ProjT2β. }
+  refine (XX $ _ $ _). clear XX. eapply λ; intro p.
+  eapply heq_trans. eapply hB. eapply eq_to_heq.
+  symmetry. unfold B2'. eapply (β@{i j1} B2).
 Defined.
 
 
-Lemma cong_lambda@{i i1 i2 j j1 j2 ij ij1 ij2} (A1 A2 : Type@{i})
-      (B1 : A1 -> Type@{j}) (B2 : A2 -> Type@{j})
-      (f1 : forall x, B1 x) (f2 : forall x, B2 x)
-      (hA : heq@{i1 i2} A1 A2)
-      (hB : forall (p : Pack@{i i1} A1 A2), heq@{j1 j2} (B1 (ProjT1 p)) (B2 (ProjT2 p)))
-      (hf : forall (p : Pack@{i i1} A1 A2), f1 (ProjT1 p) ≅ f2 (ProjT2 p))
-  : heq@{ij ij1} (fun x => f1 x) (fun x => f2 x).
+Definition congΠ'@{i i1 j j1 ij ij1} {A1 A2: Type@{i}}
+           {B1 : A1 -> Type@{j}}{B2 : A2 -> Type@{j}}
+           (pA : A1 = A2)
+           (pB : forall x, eq@{j1} (B1 x) (B2 (coe@{i i1} pA x)))
+  : @eq@{ij1} Type@{ij} (Π@{i j} A1 B1) (Π@{i j} A2 B2).
 Proof.
-  revert f1 f2 hf.
-  refine (heq_to_eq_fam'@{i i1 i2 j j1 j2 ij1 ij2 ij2} hA hB (fun A2 B2 =>   forall (f1 : forall x : A1, B1 x) (f2 : forall x : A2, B2 x), (forall p : Pack@{i i1} A1 A2, f1 (ProjT1@{i i1} p) ≅ f2 (ProjT2@{i i1} p)) -> (fun x : A1 => f1 x) ≅ (fun x : A2 => f2 x) ) _).
-  intros f1 f2 hf. apply eq_to_heq. apply funext; intro x.
-  specialize (hf (pack x x (heq_refl x))).
-  assert (hf' : f1 x ≅ f2 x). {
-    eapply heq_trans. 2:eapply heq_trans.
-    2: exact hf.
-    apply heq_apD@{i i1 j j1}. symmetry; apply ProjT1β.
-    apply heq_apD@{i i1 j j1}. apply ProjT2β. }
-  apply heq_to_eq, hf'.
+  pose (B2' := λ B2).
+  refine (@concat Type@{ij} _ (Π@{i j} A1 (fun x => B2' $ (coe@{i i1} pA x))) _ _ _).
+  2:refine (@concat Type@{ij} _ (Π@{i j} A2 (fun x => B2' $ x)) _ _ _).
+  - apply congΠ. intro x.
+    etransitivity. eapply pB. symmetry.
+    eapply (β@{i j1} B2).
+  - clearbody B2'; clear.
+    assert (Π@{ij1 ij1} (A2 ⇒ Type@{j}) (fun B2' => @eq Type@{ij} (Π@{i j} A1 (fun x : A1 => B2' $ coe@{i i1} pA x)) (Π@{i j} A2 (fun x : A2 => B2' $ x)))). {
+      clear B2'.
+      refine (J (fun A2 pA => Π@{ij1 ij1} (A2 ⇒ Type@{j}) (fun B2' : A2 ⇒ Type@{j} => @eq Type@{ij} (Π@{i j} A1 (fun x : A1 => B2' $ coe@{i i1} pA x)) (Π@{i j} A2 (fun x : A2 => B2' $ x)))) pA _).
+      apply λ; intro B. eapply congΠ.
+      intro x. refine (ap (fun x => B $ x) _). apply coeβ. }
+    refine (X $ _).
+  - apply congΠ. eapply (β@{i j1} B2).
 Defined.
 
 
-Lemma cong_app@{i i1 i2 j j1 j2 ij ij1 ij2} (A1 A2 : Type@{i})
-      (B1 : A1 -> Type@{j}) (B2 : A2 -> Type@{j})
-      (f1 : forall x, B1 x) (f2 : forall x, B2 x)
-      (u1 : A1) (u2 : A2)
-      (hA : heq@{i1 i2} A1 A2)
-      (hB : forall (p : Pack@{i i1} A1 A2), heq@{j1 j2} (B1 (ProjT1 p)) (B2 (ProjT2 p)))
-      (hf : heq@{ij ij1} f1 f2)
-      (hu : u1 ≅ u2)
-  : f1 u1 ≅ f2 u2.
+Definition coe_pV@{i i1} {A B : Type@{i}} (p : A = B) x
+  : coe p (coe@{i i1} p^ x) = x.
+Proof.
+  wrevert x. wdestruct p.
+  wintro x. etransitivity. eapply coeβ. eapply coeβ'.
+Defined.
+
+
+(* Lemma coeΠ00@{i i1 i2 j j1 j2 ij ij1 ij2} (A1 : Type@{i}) *)
+(*       (B1 B2 : A1 ⇒ Type@{j}) (f1 : Π A1 (app B1)) *)
+(*       (hB : Π A1 (fun x => B1 $ x = B2 $ x)) *)
+(*   : coe@{ij ij1} (congΠ@{i j j1 ij ij1} (fun x => hB $ x)) f1 *)
+(*     = λ@{i j} (fun x => coe (hB $ x) (f1 $ x)). *)
+(* Proof. *)
+(*   assert (hB': B1 = B2). { *)
+(*     apply funext. intro x. exact (hB $ x). } *)
+(*   simple refine (let hB'' := _ : Π@{i j1} A1 (fun x : A1 => B1 $ x = B2 $ x) in _). { *)
+(*     wintro x. exact (ap (fun B2 => B2 $ x) hB'). } *)
+(*   assert (coe@{ij ij1} (congΠ@{i j j1 ij ij1} (fun x : A1 => hB'' $ x)) f1 = λ@{i j} (fun x : A1 => coe@{j j1} (hB'' $ x) (f1 $ x))). { *)
+(*     clear hB; subst hB''. *)
+(*   revert B2 hB'; *)
+(*     match goal with *)
+(*     | |- (forall x y, ?G) => refine (fun X Y => J (fun x y => G) Y _); clear X Y *)
+(*     end. *)
+(*   etransitivity. eapply coeβ'. *)
+(*   eapply funext; intro x. *)
+(*   symmetry. etransitivity. eapply β. *)
+(*   eapply coeβ'. } *)
+(* Admitted. *)
+
+
+
+(* Lemma coeΠ0@{i i1 i2 j j1 j2 ij ij1 ij2} (A1 : Type@{i}) *)
+(*       (B1 : A1 -> Type@{j}) (B2 : A1 ⇒ Type@{j}) (f1 : Π A1 B1) *)
+(*       (hB : Π A1 (fun x => B1 x = B2 $ x)) *)
+(*   : coe@{ij ij1} (congΠ@{i j j1 ij ij1} (fun x => hB $ x)) f1 *)
+(*     = λ@{i j} (fun x => coe (hB $ x) (f1 $ x)). *)
+(* Proof. *)
+(*   simple refine (let XX :=  coeΠ00 A1 (λ B1) B2 _ _ in _). *)
+(*   - wintro x. refine (coe _ (f1 $ x)). symmetry. refine (β _ _). *)
+(*   - wintro x. etransitivity. 2: exact (hB $ x). refine (β _ _). *)
+(*   - clearbody XX. *)
+(* Abort. *)
+
+  (* assert (hB': λ B1 = B2). { *)
+  (*   apply funext. intro x. etransitivity. eapply (β B1). *)
+  (*   exact (hB $ x). } *)
+  (* simple refine (let hB'' := _ : Π@{i j1} A1 (fun x : A1 => B1 x = B2 $ x) in _). { *)
+  (*   wintro x. etransitivity. 2: exact (ap (fun B2 => B2 $ x) hB'). *)
+  (*   symmetry; apply (β B1). } *)
+  (* assert (coe@{ij ij1} (congΠ@{i j j1 ij ij1} (fun x : A1 => hB'' $ x)) f1 = λ@{i j} (fun x : A1 => coe@{j j1} (hB'' $ x) (f1 $ x))). { *)
+  (*   clear hB; subst hB''. *)
+  (* revert B2 hB'; *)
+  (*   match goal with *)
+  (*   | |- (forall x y, ?G) => refine (fun X Y => J (fun x y => G) Y _); clear X Y *)
+  (*   end. *)
+
+  (* match goal with *)
+  (* | |- coe ?XX _ = _ => set XX *)
+  (* end. *)
+
+
+
+(* Lemma coeΠ0@{i i1 i2 j j1 j2 ij ij1 ij2} (A1 A2 : Type@{i}) *)
+(*       (B1 : A1 -> Type@{j}) (B2 : A2 ⇒ Type@{j}) (f1 : Π A1 B1) *)
+(*       (hA : A1 = A2) (hB : Π A1 (fun x => B1 x = B2 $ (coe@{i i1} hA x))) *)
+(*   : coe@{ij ij1} (congΠ'@{i i1 j j1 ij ij1} hA (fun x => hB $ x)) f1 *)
+(*     = λ@{i j} (fun x => coe@{j j1} (hB $ (coe@{i i1} hA^ x) *)
+(*                @ ap@{i j1} (fun x => B2 $ x) (coe_pV@{i i1} hA x)) (f1 $ coe@{i i1} hA^ x)). *)
+(* Proof. *)
+(*   wrevert hB. *)
+(*   wrevert B2. *)
+(*   wdestruct A2 hA. *)
+(*   wintro B2. wintro hB. *)
+(*   assert (hB': λ B1 = B2). { *)
+(*     apply funext. intro x. etransitivity. eapply (β B1). *)
+(*     etransitivity. exact (hB $ x). *)
+(*     refine (ap (fun x => B2 $ x) _). apply coeβ. } *)
+(*   simple refine (let hB'' := _ : Π@{i j1} A1 (fun x : A1 => B1 x = B2 $ coe@{i i1} 1 x) *)
+(*                  in _). { *)
+(*     wintro x. etransitivity. *)
+(*     2: exact (ap (fun f => f $ _) hB'). symmetry. etransitivity. *)
+(*     eapply (β B1). eapply ap, coeβ. } *)
+(*   assert (coe@{ij ij1} (congΠ'@{i i1 j j1 ij ij1} 1 (fun x : A1 => hB'' $ x)) f1 = λ@{i j} (fun x : A1 => coe@{j j1} (hB'' $ coe@{i i1} 1^ x @ ap@{i j1} (fun x0 : A1 => B2 $ x0) (coe_pV@{i i1} 1 x)) (f1 $ coe@{i i1} 1^ x))). { *)
+(*     clear hB. subst hB''. *)
+(*   revert B2 hB'; *)
+(*     match goal with *)
+(*     | |- (forall x y, ?G) => refine (fun X Y => J (fun x y => G) Y _); clear X Y *)
+(*     end. *)
+  
+(*   match goal with *)
+(*   | |- coe ?XX _ = _ => set XX *)
+(*   end. *)
+(* Abort. *)
+
+
+
+
+(* Lemma coeΠ@{i i1 i2 j j1 j2 ij ij1 ij2} (A1 A2 : Type@{i}) *)
+(*       (B1 : A1 -> Type@{j}) (B2 : A2 -> Type@{j}) *)
+(*       (f1 : Π A1 B1) (f2 : Π A2 B2) *)
+(*       (hA : A1 = A2) (hB : forall x : A1, B1 x = B2 (coe@{i i1} hA x)) *)
+(*       (hB' : forall x, B1 (coe@{i i1} hA^ x) = B2 x := fun x => hB _ @ ap B2 (coe_pV hA x)) *)
+(*   : coe@{ij ij1} (congΠ'@{i i1 j j1 ij ij1} hA hB) f1 *)
+(*     = λ (fun x => coe (hB' x) (f1 $ (coe hA^ x))). *)
+(* Proof. *)
+(*   subst hB'. cbn. *)
+(*   pose (hB' := λ@{j1 ij1} hB). *)
+(*   transitivity (coe@{ij ij1} (congΠ'@{i i1 j j1 ij ij1} hA (fun x => hB' $ x)) f1). *)
+(*   admit. *)
+(*   clearbody hB'; clear. *)
+
+  (* refine (@App@{ij1 ij1} _ (fun hB' => coe@{ij ij1} (congΠ'@{i i1 j j1 ij ij1} 
+hA (fun x : A1 => hB' $ x)) f1 = f2) _ hB'). clear. *)
+  (* refine (@App@{ij1 ij1} _ (fun f2 =>  Π@{ij1 ij1} (Π@{j1 ij1} A1 (fun x : A1 => B1 x = B2 (coe@{i i1} hA x))) (fun hB' : Π@{j1 ij1} A1 (fun x : A1 => B1 x = B2 (coe@{i i1} hA x)) => coe@{ij ij1} (congΠ'@{i i1 j j1 ij ij1} hA (fun x : A1 => hB' $ x)) f1 = f2)) *)
+  (*             _ f2). clear. *)
+  (* refine (@App@{ij1 ij1} _ (fun B2 => Π@{ij1 ij1} (Π@{i j} A2 B2) (fun f2 : Π@{i j} A2 B2 => Π@{ij1 ij1} (Π@{j1 ij1} A1 (fun x : A1 => B1 x = B2 (coe@{i i1} hA x))) (fun hB' : Π@{j1 ij1} A1 (fun x : A1 => B1 x = B2 (coe@{i i1} hA x)) => coe@{ij ij1} (congΠ'@{i i1 j j1 ij ij1} hA (fun x : A1 => hB' $ x)) f1 = f2))) _ B2) *)
+
+(*   refine (J (fun A2 hA =>  Π@{ij1 ij1} (Π@{j1 ij1} A1 (fun x : A1 => B1 x = B2 (coe@{i i1} hA x))) (fun hB'0 : Π@{j1 ij1} A1 (fun x : A1 => B1 x = B2 (coe@{i i1} hA x)) => coe@{ij ij1} (congΠ'@{i i1 j j1 ij ij1} hA (fun x : A1 => hB'0 $ x)) f1 = f2)) hA _). *)
+(* )) *)
+
+Lemma heq_fam_to_eq (A1 : Type) (B1 B2 : A1 ⇒ Type)
+      (hB : Π (Pack A1 A1) (fun p => B1 $ ProjT1 p ≅ B2 $ ProjT2 p))
+  : B1 = B2.
+Proof.
+  apply funext; intro x.
+  refine (_ @ heq_to_eq (hB $ (pack x x E1)) @ _).
+  refine (ap (fun x => B1 $ x) _). symmetry; apply ProjT1β.
+  refine (ap (fun x => B2 $ x) _). apply ProjT2β.
+Defined.
+    
+
+
+(* Lemma cong_lambda0@{i i1 i2 j j1 j2 ij ij1 ij2} (A1 A2 : Type@{i}) *)
+(*       (B1 : A1 ⇒ Type@{j}) (B2 : A2 ⇒ Type@{j}) *)
+(*       (f1 : Π A1 (fun x => B1 $ x)) (f2 : Π A2 (fun x => B2 $ x)) *)
+(*       (hA : heq@{i1 i2} A1 A2) *)
+(*       (hB : Π (Pack@{i i1} A1 A2) (fun p => heq@{j1 j2} (B1 $ (ProjT1 p)) (B2 $ (ProjT2 p)))) *)
+(*       (hf : Π (Pack@{i i1} A1 A2) (fun p => f1 $ (ProjT1 p) ≅ f2 $ (ProjT2 p))) *)
+(*   : heq@{ij ij1} f1 f2. *)
+Lemma cong_lambda0 (A1 A2 : Type)
+      (B1 : A1 ⇒ Type) (B2 : A2 ⇒ Type)
+      (f1 : Π A1 (fun x => B1 $ x)) (f2 : Π A2 (fun x => B2 $ x))
+      (hA : heq A1 A2)
+      (hB : Π (Pack A1 A2) (fun p => heq (B1 $ (ProjT1 p)) (B2 $ (ProjT2 p))))
+      (hf : Π (Pack A1 A2) (fun p => f1 $ (ProjT1 p) ≅ f2 $ (ProjT2 p)))
+  : heq f1 f2.
 Proof.
   apply heq_to_eq in hA.
-  revert B2 hB f2 hf u2 hu.
-  refine (transport@{i1 ij1} (fun A2 : Type@{i} =>  forall B2 : A2 -> Type@{j},
-  (forall p : Pack@{i i1} A1 A2, B1 (ProjT1@{i i1} p) ≅ B2 (ProjT2@{i i1} p)) ->
-  forall (f2 : forall x : A2, B2 x), f1 ≅ f2 -> forall (u2 : A2), u1 ≅ u2 -> f1 u1 ≅ f2 u2) hA _).
-  clear A2 hA; intros B2 hB.
-  apply heq_to_eq_fam in hB.
-  refine (transport@{ij1 ij2} (fun B2 : A1 -> Type@{j} =>  forall (f2 : forall x : A1, B2 x),
-  f1 ≅ f2 -> forall u2 : A1, u1 ≅ u2 -> f1 u1 ≅ f2 u2) hB _).
-  clear hB B2; intros f2 hf.
-  apply heq_to_eq in hf.
-  refine (transport@{ij ij1} (fun f2 => forall u2 : A1, u1 ≅ u2 -> f1 u1 ≅ f2 u2) hf _).
-  clear f2 hf; intros u2 hu. 
-  apply heq_to_eq in hu.
-  refine (transport@{ij ij1} (fun u2 => f1 u1 ≅ f1 u2) hu _).
-  apply heq_refl.
+  wrevert hf f2 hB B2. wdestruct hA. wintro B2 hB.
+  apply heq_fam_to_eq in hB. wdestruct hB.
+  wintro f2 hf. apply eq_to_heq, funext; intro x.
+  apply heq_to_eq.
+  refine (_ E@ (hf $ (pack x x E1)) E@ _).
+  unshelve eexists. exact (ap (fun x => B1 $ x) (ProjT1β _ _ _)^).
+  (* set (ProjT1β@{i i1} x x E1)^. *)
+  (* set (y := ProjT1@{i i1} (pack@{i i1} x x E1)) in *. *)
+  (* clearbody e y. wdestruct y e. apply coeβ'. *)
+  (* set (ProjT2β@{i i1} x x E1)^. *)
+  (* set (y := ProjT2@{i i1} (pack@{i i1} x x E1)) in *. *)
+  set (ProjT1β x x E1)^.
+  set (y := ProjT1 (pack x x E1)) in *.
+  clearbody e y. wdestruct e. apply coeβ'.
+  set (ProjT2β x x E1)^.
+  set (y := ProjT2 (pack x x E1)) in *.
+  clearbody e y. wdestruct e. exact E1.
 Defined.
+
+
+(* Lemma cong_lambda@{i i1 i2 j j1 j2 ij ij1 ij2} (A1 A2 : Type@{i}) *)
+(*       (B1 : A1 -> Type@{j}) (B2 : A2 -> Type@{j}) *)
+(*       (f1 : forall x, B1 x) (f2 : forall x, B2 x) *)
+(*       (hA : heq@{i1 i2} A1 A2) *)
+(*       (hB : forall (p : Pack@{i i1} A1 A2), heq@{j1 j2} (B1 (ProjT1 p)) (B2 (ProjT2 p))) *)
+(*       (hf : forall (p : Pack@{i i1} A1 A2), f1 (ProjT1 p) ≅ f2 (ProjT2 p)) *)
+(*   : heq@{ij ij1} (λ f1) (λ f2). *)
+Lemma cong_lambda (A1 A2 : Type)
+      (B1 : A1 -> Type) (B2 : A2 -> Type)
+      (f1 : forall x, B1 x) (f2 : forall x, B2 x)
+      (hA : heq A1 A2)
+      (hB : forall (p : Pack A1 A2), heq (B1 (ProjT1 p)) (B2 (ProjT2 p)))
+      (hf : forall (p : Pack A1 A2), f1 (ProjT1 p) ≅ f2 (ProjT2 p))
+  : heq (λ f1) (λ f2).
+Proof.
+  simple refine (let XX := cong_lambda0 A1 A2 (λ B1) (λ B2) (λ (fun x => coe (β B1 x)^ (f1 x))) (λ (fun x => coe (β B2 x)^ (f2 x))) hA _ (* hB *) _ (* hf *) in _).
+  - wintro p. refine (_ E@ hB p E@ _).
+    all: eapply eq_to_heq; beta.
+  - wintro p. refine (_ E@ hf p E@ _).
+    unshelve eexists. beta.
+    refine (ap (coe _) _ @ _). beta. apply coe_pV.
+    unshelve eexists. beta.
+    etransitivity. 2: refine (β _ _)^. reflexivity.
+  - refine (_ E@ XX E@ _); clear. 
+    + apply heq_sym. unshelve eexists.
+      apply congΠ. intro x; refine (β _ _).
+      etransitivity. eapply congΠβ. cbn.
+      apply funext; intro x. refine (β _ _ @ _ @ (β _ _)^).
+      refine (ap (coe _) _ @ _). refine (β _ _). apply coe_pV.
+    + apply heq_sym. unshelve eexists.
+      apply congΠ. intro x; refine (β _ _)^.
+      etransitivity. eapply congΠβ. cbn.
+      apply funext; intro x. refine (β _ _ @ _ @ (β _ _)^).
+      refine (ap (coe _) _). refine (β _ _).
+Defined.
+
+Lemma cong_app0 (A1 A2 : Type)
+      (B1 : A1 ⇒ Type) (B2 : A2 ⇒ Type)
+      (f1 : Π A1 (app B1)) (f2 : Π A2 (app B2))
+      (u1 : A1) (u2 : A2)
+      (hA : heq A1 A2)
+      (hB : Π (Pack A1 A2) (fun p => heq (B1 $ (ProjT1 p)) (B2 $ (ProjT2 p))))
+      (hf : heq f1 f2)
+      (hu : u1 ≅ u2)
+  : f1 $ u1 ≅ f2 $ u2.
+Proof.
+  wrevert hu u2 hf f2 hB B2.
+    apply heq_to_eq in hA. wdestruct hA. wintro B2 hB.
+  apply heq_fam_to_eq in hB. wdestruct hB.
+  wintro f2 hf. apply heq_to_eq in hf. wdestruct hf.
+  wintro u2 hu. apply heq_to_eq in hu. wdestruct hu.
+  exact E1.
+Defined.
+
+(* Lemma cong_app@{i i1 i2 j j1 j2 ij ij1 ij2} (A1 A2 : Type@{i}) *)
+(*       (B1 : A1 -> Type@{j}) (B2 : A2 -> Type@{j}) *)
+(*       (f1 : Π A1 B1) (f2 : Π A2 B2) *)
+(*       (u1 : A1) (u2 : A2) *)
+(*       (hA : heq@{i1 i2} A1 A2) *)
+(*       (hB : forall (p : Pack@{i i1} A1 A2), heq@{j1 j2} (B1 (ProjT1 p)) (B2 (ProjT2 p))) *)
+(*       (hf : heq@{ij ij1} f1 f2) *)
+(*       (hu : u1 ≅ u2) *)
+(*   : f1 $ u1 ≅ f2 $ u2. *)
+Lemma cong_app (A1 A2 : Type)
+      (B1 : A1 -> Type) (B2 : A2 -> Type)
+      (f1 : Π A1 B1) (f2 : Π A2 B2)
+      (u1 : A1) (u2 : A2)
+      (hA : heq A1 A2)
+      (hB : forall (p : Pack A1 A2), heq (B1 (ProjT1 p)) (B2 (ProjT2 p)))
+      (hf : heq f1 f2)
+      (hu : u1 ≅ u2)
+  : f1 $ u1 ≅ f2 $ u2.
+Proof.
+  simple refine (let XX := cong_app0 A1 A2 (λ B1) (λ B2) _ _ u1 u2 hA _ (* hB *) _ (* hf *) hu in _).
+  - refine (λ (fun x => coe (β B1 x)^ (f1 $ x))).
+  - refine (λ (fun x => coe (β B2 x)^ (f2 $ x))).
+  - wintro p. refine (_ E@ hB p E@ _).
+    eapply eq_to_heq. refine (β _ _).
+    eapply eq_to_heq. refine (β _ _)^.
+  - refine (_ E@ hf E@ _).
+    unshelve eexists. apply congΠ. intro; refine (β _ _).
+    etransitivity. apply congΠβ. apply funext; intro x.
+    refine (β _ _ @ _). refine (ap (coe _) _ @ _).
+    refine (β _ _). apply coe_pV.
+    unshelve eexists. apply congΠ. intro; refine (β _ _)^.
+    etransitivity. apply congΠβ. reflexivity.
+  - refine (_ E@ XX E@ _); clear XX.
+    + eapply heq_trans. 2: apply eq_to_heq; refine (β _ _)^.
+      apply heq_coe.
+    + eapply heq_trans. apply eq_to_heq; refine (β _ _).
+      apply heq_sym, heq_coe.
+Defined.
+
+
+Axiom congΣ@{i j j1 ij ij1} : forall {A : Type@{i}}{B B': A -> Type@{j}},
+    (forall x, eq@{j1} (B x) (B' x)) -> @eq@{ij1} Type@{ij} (sigT@{i j} B) (sigT@{i j} B').
+
+Lemma congΣβ@{i i1 i2 j j1 j2 ij ij1 ij2} (A1 : Type@{i})
+      (B1 B2 : A1 -> Type@{j}) u v
+      (hB : forall x, B1 x = B2 x)
+  : coe@{ij ij1} (congΣ@{i j j1 ij ij1} hB) (u; v)
+    = (u; coe (hB _) v).
+Proof.
+Admitted.
 
 Lemma cong_sum@{i i1 i2 j j1 j2 ij ij1 ij2} (A1 A2 : Type@{i})
       (B1 : A1 -> Type@{j}) (B2 : A2 -> Type@{j})
@@ -339,112 +675,208 @@ Lemma cong_sum@{i i1 i2 j j1 j2 ij ij1 ij2} (A1 A2 : Type@{i})
       (hB : forall (p : Pack@{i i1} A1 A2), heq@{j1 j2} (B1 (ProjT1 p)) (B2 (ProjT2 p)))
   : @heq@{ij1 ij2} Type@{ij} (sigT B1) Type@{ij} (sigT B2).
 Proof.
-  exists 1. etransitivity. eapply coeβ.
-  apply heq_to_eq in hA.
-  revert B2 hB.
-  refine (transport@{i1 ij1} (fun A2 : Type@{i} => forall B2 : A2 -> Type@{j},
-                     (forall p, B1 (ProjT1 p) ≅ B2 (ProjT2 p)) ->
-                     @eq Type@{ij} (sigT B1) (sigT B2)) hA _).
-  intros B2 hB. apply heq_to_eq_fam in hB.
-  refine (ap@{ij1 _} (B:=Type@{ij})(fun B : A1 -> Type@{j} => sigT B) hB).
+  apply heq_to_eq in hA. apply eq_to_heq.
+  pose (B2' := λ@{i j1} B2).
+  refine (@concat Type@{ij} _ (sigT@{i j} (app B2')) _ _ _).
+  2: apply congΣ@{i j j1 ij ij1}; intro x; apply (β@{i j1} B2 x).
+  assert (hB': (Π@{ij1 ij1} (Pack@{i i1} A1 A2) (fun p => B1 (ProjT1@{i i1} p) ≅ B2' $ (ProjT2@{i i1} p)))). {
+    wintro p. refine (hB p E@ _). apply eq_to_heq.
+    refine (β _ _)^. }
+  clearbody B2'; clear B2 hB. wrevert hB'. wrevert B2'.
+  let e := hA in
+  match type of e with
+  | _ = ?y => 
+  revert y e;
+    match goal with
+    | |- (forall y e, ?G) => let X := fresh in let Y := fresh in
+                      refine (fun X Y => J@{i1 ij1} (fun y e => G) Y _); clear X Y
+    end end.
+  refine (λ@{i ij1} (fun B2 => _)). wintro hB. apply congΣ.
+  intro x. pose proof (hB $ (pack@{i i1} x x (heq_refl x))).
+  cbn in *. apply heq_to_eq in X. etransitivity. etransitivity.
+  2: exact X. all: apply ap.
+  symmetry. apply ProjT1β. apply ProjT2β.
 Defined.
 
-Lemma cong_pair@{i i1 i2 j j1 j2 ij ij1 ij2} (A1 A2 : Type@{i})
-      (B1 : A1 -> Type@{j}) (B2 : A2 -> Type@{j})
+Lemma cong_pair0 (A1 A2 : Type)
+      (B1 : A1 ⇒ Type) (B2 : A2 ⇒ Type)
+      (u1 : A1) (u2 : A2) (v1 : B1 $ u1) (v2 : B2 $ u2)
+      (hA : heq A1 A2)
+      (hB : Π (Pack A1 A2) (fun p => heq (B1 $ (ProjT1 p)) (B2 $ (ProjT2 p))))
+      (hu : u1 ≅ u2) (hv : v1 ≅ v2)
+  : (existT _ u1 v1) ≅ (existT _ u2 v2).
+Proof.
+  wrevert hv v2 hu u2 hB B2.
+  apply heq_to_eq in hA. wdestruct hA. wintro B2 hB.
+  apply heq_fam_to_eq in hB. wdestruct hB.
+  wintro u2 hu. apply heq_to_eq in hu; wdestruct hu.
+  wintro v2 hv. apply heq_to_eq in hv; wdestruct hv.
+  exact E1.
+Defined.
+
+Lemma eq_sigma {A} (B : A -> Type) {x x' : A} {y : B x} {y' : B x'}
+      (e1 : x = x') (e2 : e1 # y = y')
+  : (x; y) = (x'; y').
+Proof.
+  wrevert e2 y'. wdestruct e1.
+  wintro y' e2. pose proof ((transportβ B y)^ @ e2).
+  clear e2. wdestruct X. reflexivity.
+Defined.
+
+(* Lemma cong_pair@{i i1 i2 j j1 j2 ij ij1 ij2} (A1 A2 : Type@{i}) *)
+(*       (B1 : A1 -> Type@{j}) (B2 : A2 -> Type@{j}) *)
+(*       (u1 : A1) (u2 : A2) (v1 : B1 u1) (v2 : B2 u2) *)
+(*       (hA : heq@{i1 i2} A1 A2) *)
+(*       (hB : forall (p : Pack@{i i1} A1 A2), heq@{j1 j2} (B1 (ProjT1 p)) (B2 (ProjT2 p))) *)
+(*       (hu : u1 ≅ u2) (hv : v1 ≅ v2) *)
+(*   : heq@{ij ij1} (existT B1 u1 v1) (existT B2 u2 v2). *)
+Lemma cong_pair (A1 A2 : Type)
+      (B1 : A1 -> Type) (B2 : A2 -> Type)
       (u1 : A1) (u2 : A2) (v1 : B1 u1) (v2 : B2 u2)
-      (hA : heq@{i1 i2} A1 A2)
-      (hB : forall (p : Pack@{i i1} A1 A2), heq@{j1 j2} (B1 (ProjT1 p)) (B2 (ProjT2 p)))
-  : u1 ≅ u2 ->
-    v1 ≅ v2 ->
-    heq@{ij ij1} (existT B1 u1 v1) (existT B2 u2 v2).
+      (hA : heq A1 A2)
+      (hB : forall (p : Pack A1 A2), heq (B1 (ProjT1 p)) (B2 (ProjT2 p)))
+      (hu : u1 ≅ u2) (hv : v1 ≅ v2)
+  : heq (existT B1 u1 v1) (existT B2 u2 v2).
 Proof.
-  revert B2 hB u2 v2.
-apply heq_to_eq in hA.
-  refine (transport@{i1 ij1} (fun A2 : Type@{i} =>  forall B2 : A2 -> Type@{j},
-  (forall p : Pack@{i i1} A1 A2, B1 (ProjT1@{i i1} p) ≅ B2 (ProjT2@{i i1} p)) ->
-  forall (u2 : A2) (v2 : B2 u2), u1 ≅ u2 -> v1 ≅ v2 -> (u1; v1) ≅ (u2; v2)) hA _).
-  clear A2 hA; intros B2 hB.
-  apply heq_to_eq_fam in hB.
-  refine (transport@{ij1 ij2} (fun B2 : A1 -> Type@{j} => forall (u2 : A1) (v2 : B2 u2),
-                                 u1 ≅ u2 -> v1 ≅ v2 -> (u1; v1) ≅ (u2; v2)) hB _).
-  clear hB B2; intros u2 v2 hu; revert v2.
-  apply heq_to_eq in hu.
-  refine (transport@{ij ij1} (fun u2 => forall v2 : B1 u2, v1 ≅ v2 -> (u1; v1) ≅ (u2; v2)) hu _).
-  clear u2 hu; intros v2 hv. 
-  apply heq_to_eq in hv.
-  refine (transport@{ij ij1} (fun v2 => (u1; v1) ≅ (u1; v2)) hv _).
-  apply heq_refl.
+  simple refine (let XX := cong_pair0 A1 A2 (λ B1) (λ B2) u1 u2 (coe (β _ _)^ v1) (coe (β _ _)^ v2) hA _ hu _ in _ E@ XX E@ _).
+  - wintro p. refine (eq_to_heq (β _ _) E@ _ E@ eq_to_heq (β _ _)^).
+    apply hB.
+  - refine (_^E E@ hv E@ _); apply heq_coe; clear.
+  - unshelve eexists. apply congΣ. intro x; refine (β _ _)^.
+    etransitivity. apply congΣβ. reflexivity. 
+  - eapply heq_sym. unshelve eexists. apply congΣ. intro x; refine (β _ _)^.
+    etransitivity. apply congΣβ. reflexivity. 
 Defined.
 
-Lemma cong_pi1@{i i1 i2 j j1 j2 ij ij1 ij2} (A1 A2 : Type@{i})
-      (B1 : A1 -> Type@{j}) (B2 : A2 -> Type@{j})
-      (p1 : sigT B1) (p2 : sigT B2)
-      (hA : heq@{i1 i2} A1 A2)
-      (hB : forall (p : Pack@{i i1} A1 A2), heq@{j1 j2} (B1 (ProjT1 p)) (B2 (ProjT2 p)))
-  : heq@{ij ij1} p1 p2 -> p1.1 ≅ p2.1.
+Lemma cong_pi10 (A1 A2 : Type) (B1 : A1 ⇒ Type) (B2 : A2 ⇒ Type)
+      (p1 : sigT (app B1)) (p2 : sigT (app B2))
+      (hA : heq A1 A2)
+      (hB : Π (Pack A1 A2) (fun p => heq (B1 $ (ProjT1 p)) (B2 $ (ProjT2 p))))
+      (hp : p1 ≅ p2)
+  : p1.1 ≅ p2.1.
 Proof.
-  apply heq_to_eq in hA.
-  revert B2 hB p2.
-  refine (transport@{i1 ij1} (fun A2 : Type@{i} =>  forall B2 : A2 -> Type@{j},
-    (forall p : Pack@{i i1} A1 A2, B1 (ProjT1@{i i1} p) ≅ B2 (ProjT2@{i i1} p)) ->
-  forall (p2 : {x : _ & B2 x}), p1 ≅ p2 -> p1.1 ≅ p2.1) hA _).
-  clear A2 hA; intros B2 hB.
-  apply heq_to_eq_fam in hB.
-  refine (transport@{ij1 ij2} (fun B2 : A1 -> Type@{j} => forall (p2 : {x : A1 & B2 x}), p1 ≅ p2 -> p1.1 ≅ p2.1) hB _).
-  clear hB B2; intros p2 hp.
-  apply heq_to_eq in hp.
-  refine (transport@{ij ij1} (fun p2 => p1.1 ≅ p2.1) hp _).
-  apply heq_refl.
+  wrevert hp p2 hB B2.
+  apply heq_to_eq in hA. wdestruct hA. wintro B2 hB.
+  apply heq_fam_to_eq in hB. wdestruct hB.
+  wintro p2 hp. apply heq_to_eq in hp; wdestruct hp.
+  exact E1.
 Defined.
 
-Lemma cong_pi2@{i i1 i2 j j1 j2 ij ij1 ij2} (A1 A2 : Type@{i})
-      (B1 : A1 -> Type@{j}) (B2 : A2 -> Type@{j})
+(* Lemma cong_pi1@{i i1 i2 j j1 j2 ij ij1 ij2} (A1 A2 : Type@{i}) *)
+(*       (B1 : A1 -> Type@{j}) (B2 : A2 -> Type@{j}) *)
+(*       (p1 : sigT B1) (p2 : sigT B2) *)
+(*       (hA : heq@{i1 i2} A1 A2) *)
+(*       (hB : forall (p : Pack@{i i1} A1 A2), heq@{j1 j2} (B1 (ProjT1 p)) (B2 (ProjT2 p))) *)
+(*       (hp : heq@{ij ij1} p1 p2) *)
+(*   : p1.1 ≅ p2.1. *)
+Lemma cong_pi1 (A1 A2 : Type)
+      (B1 : A1 -> Type) (B2 : A2 -> Type)
       (p1 : sigT B1) (p2 : sigT B2)
-      (hA : heq@{i1 i2} A1 A2)
-      (hB : forall (p : Pack@{i i1} A1 A2), heq@{j1 j2} (B1 (ProjT1 p)) (B2 (ProjT2 p)))
-  : heq@{ij ij1} p1 p2 -> p1.2 ≅ p2.2.
+      (hA : heq A1 A2)
+      (hB : forall (p : Pack A1 A2), heq (B1 (ProjT1 p)) (B2 (ProjT2 p)))
+      (hp : p1 ≅ p2)
+  : p1.1 ≅ p2.1.
 Proof.
-  apply heq_to_eq in hA.
-  revert B2 hB p2.
-  refine (transport@{i1 ij1} (fun A2 : Type@{i} =>  forall B2 : A2 -> Type@{j},
-    (forall p : Pack@{i i1} A1 A2, B1 (ProjT1@{i i1} p) ≅ B2 (ProjT2@{i i1} p)) ->
-  forall (p2 : {x : _ & B2 x}), p1 ≅ p2 -> p1.2 ≅ p2.2) hA _).
-  clear A2 hA; intros B2 hB.
-  apply heq_to_eq_fam in hB.
-  refine (transport@{ij1 ij2} (fun B2 : A1 -> Type@{j} => forall (p2 : {x : A1 & B2 x}), p1 ≅ p2 -> p1.2 ≅ p2.2) hB _).
-  clear hB B2; intros p2 hp.
-  apply heq_to_eq in hp.
-  refine (transport@{ij ij1} (fun p2 => p1.2 ≅ p2.2) hp _).
-  apply heq_refl.
+  simple refine (let XX := cong_pi10 A1 A2 (λ B1) (λ B2) _ _ hA _ _ in _ E@ XX E@ _).
+  - refine (coe _ p1). apply congΣ. intro; beta.
+  - refine (coe _ p2). apply congΣ. intro; beta.
+  - wintro p. refine (_ E@ hB p E@ _); apply eq_to_heq.
+    refine (β _ _). refine (β _ _)^.
+  - refine (_^E E@ hp E@ _); apply heq_coe.
+  - clear. apply eq_to_heq. symmetry. etransitivity.
+    eapply ap. etransitivity. apply ap. 2: apply congΣβ.
+    symmetry; apply Ση. apply projT1β.
+  - clear. apply eq_to_heq. etransitivity.
+    eapply ap. etransitivity. apply ap. 2: apply congΣβ.
+    symmetry; apply Ση. apply projT1β.
 Defined.
+
+
+Lemma cong_pi20 (A1 A2 : Type) (B1 : A1 ⇒ Type) (B2 : A2 ⇒ Type)
+      (p1 : sigT (app B1)) (p2 : sigT (app B2))
+      (hA : heq A1 A2)
+      (hB : Π (Pack A1 A2) (fun p => heq (B1 $ (ProjT1 p)) (B2 $ (ProjT2 p))))
+      (hp : p1 ≅ p2)
+  : p1.2 ≅ p2.2.
+Proof.
+  wrevert hp p2 hB B2.
+  apply heq_to_eq in hA. wdestruct hA. wintro B2 hB.
+  apply heq_fam_to_eq in hB. wdestruct hB.
+  wintro p2 hp. apply heq_to_eq in hp; wdestruct hp.
+  exact E1.
+Defined.
+
+Definition Eap {A} {B : A -> Type} (f : forall x, B x) {x x'} (e : x = x')
+  : f x ≅ f x'.
+Admitted.
+
+
+(* Lemma cong_pi2@{i i1 i2 j j1 j2 ij ij1 ij2} (A1 A2 : Type@{i}) *)
+(*       (B1 : A1 -> Type@{j}) (B2 : A2 -> Type@{j}) *)
+(*       (p1 : sigT B1) (p2 : sigT B2) *)
+(*       (hA : heq@{i1 i2} A1 A2) *)
+(*       (hB : forall (p : Pack@{i i1} A1 A2), heq@{j1 j2} (B1 (ProjT1 p)) (B2 (ProjT2 p))) *)
+(*   : heq@{ij ij1} p1 p2 -> p1.2 ≅ p2.2. *)
+Lemma cong_pi2 (A1 A2 : Type)
+      (B1 : A1 -> Type) (B2 : A2 -> Type)
+      (p1 : sigT B1) (p2 : sigT B2)
+      (hA : heq A1 A2)
+      (hB : forall (p : Pack A1 A2), heq (B1 (ProjT1 p)) (B2 (ProjT2 p)))
+      (hp : p1 ≅ p2)
+  : p1.2 ≅ p2.2.
+Proof.
+  simple refine (let XX := cong_pi20 A1 A2 (λ B1) (λ B2) _ _ hA _ _ in _ E@ XX E@ _).
+  - refine (coe _ p1). apply congΣ. intro; beta.
+  - refine (coe _ p2). apply congΣ. intro; beta.
+  - wintro p. refine (_ E@ hB p E@ _); apply eq_to_heq.
+    refine (β _ _). refine (β _ _)^.
+  - refine (_^E E@ hp E@ _); apply heq_coe.
+  - clear. symmetry.
+    pose proof (Ση _ p1). set (p1' := (p1.1; p1.2)) in *.
+    transitivity (coe (congΣ (fun x : A1 => (β B1 x)^)) p1').2.
+    clearbody p1'. wdestruct X. reflexivity.
+    subst p1'; clear X.
+    pose proof (congΣβ _ _ _ p1.1 p1.2 (fun x => (β B1 x)^))^.
+    set (Y := coe (congΣ (fun x : A1 => (β B1 x)^)) (p1.1; p1.2)) in *.
+    etransitivity. clearbody Y. wdestruct X. reflexivity.
+    etransitivity. apply eq_to_heq. eapply projT2β'.
+    symmetry. etransitivity. 2: eapply heq_transport.
+    eapply heq_coe.
+  - clear. pose proof (Ση _ p2). set (p2' := (p2.1; p2.2)) in *.
+    transitivity (coe (congΣ (fun x : A2 => (β B2 x)^)) p2').2.
+    clearbody p2'. wdestruct X. reflexivity.
+    subst p2'; clear X.
+    pose proof (congΣβ _ _ _ p2.1 p2.2 (fun x => (β B2 x)^))^.
+    set (Y := coe (congΣ (fun x : A2 => (β B2 x)^)) (p2.1; p2.2)) in *.
+    etransitivity. clearbody Y. wdestruct X. reflexivity.
+    etransitivity. apply eq_to_heq. eapply projT2β'.
+    symmetry. etransitivity. 2: eapply heq_transport.
+    eapply heq_coe.
+Defined.
+
 
 Lemma cong_eq@{i i1 i2} (A1 A2 : Type@{i})
       (u1 v1 : A1) (u2 v2 : A2)
       (hA : heq@{i1 i2} A1 A2)
-  : u1 ≅ u2 -> v1 ≅ v2 -> (u1 = v1) ≅ (u2 = v2).
+      (hu : u1 ≅ u2) (hv :  v1 ≅ v2)
+  : (u1 = v1) ≅ (u2 = v2).
 Proof.
   apply heq_to_eq in hA.
-  revert u2 v2.
-  refine (transport (fun A2 : Type@{i} => forall u2 v2 : A2, u1 ≅ u2 -> v1 ≅ v2 -> (u1 = v1) ≅ (u2 = v2)) hA _).
-  clear A2 hA. intros u2 v2 hu; revert v2.
-  apply heq_to_eq in hu.
-  refine (transport (fun u2 => forall v2 : A1, v1 ≅ v2 -> (u1 = v1) ≅ (u2 = v2)) hu _).
-  intros v2 hv. apply heq_to_eq in hv.
-  refine (transport (fun v2 => (u1 = v1) ≅ (u1 = v2)) hv _).
-  apply heq_refl.
+  wrevert hv v2 hu u2. wdestruct hA.
+  wintro u2 hu; apply heq_to_eq in hu; wdestruct hu.
+  wintro v2 hv; apply heq_to_eq in hv; wdestruct hv.
+  reflexivity.
 Defined.
 
 Lemma cong_refl@{i i1 i2} (A1 A2 : Type@{i})
       (u1 : A1) (u2 : A2)
-      (hA : heq@{i1 i2} A1 A2)
-  : u1 ≅ u2 -> @eq_refl A1 u1 ≅ @eq_refl A2 u2.
+      (hA : heq@{i1 i2} A1 A2) (hu : u1 ≅ u2)
+  : @eq_refl A1 u1 ≅ @eq_refl A2 u2.
 Proof.
   apply heq_to_eq in hA.
-  revert u2. 
-  refine (transport (fun A2 : Type@{i} => forall u2 : A2, u1 ≅ u2 -> @eq_refl A1 u1 ≅ @eq_refl A2 u2) hA _).
-  clear A2 hA; intros u2 hu. apply heq_to_eq in hu.
-  refine (transport (fun u2 => @eq_refl A1 u1 ≅ @eq_refl A1 u2) hu _).
-  apply heq_refl.
+  wrevert hu u2. wdestruct hA.
+  wintro u2 hu; apply heq_to_eq in hu; wdestruct hu.
+  reflexivity.
 Defined.
 
 
